Compose

simple/proofs.v
@@ -1,6 +1,21 @@
 Set Implicit Arguments.
 Set Asymmetric Patterns.
 
+Definition compose (A B C : Set) (f : B -> C) (g : A -> B) := fun x => f (g x).
+Notation "f 'o' g" := (compose f g) (at level 80, right associativity).
+
+Inductive option (T : Set) : Set :=
+| SOME : T -> option T
+| NONE : option T.
+
+Definition compose' (A B C : Set)(f : B -> option C) (g : A -> option B) : (A -> option C) :=
+  fun a => match g a with
+           | NONE => NONE C
+           | SOME b => f b
+           end.
+
+Notation "f 'oo' g" := (compose' f g) (at level 80, right associativity).
+
 Inductive bool : Set := true : bool | false : bool.
 
 Definition and (b1 b2 : bool) : bool :=
@@ -16,21 +31,35 @@ Inductive list (T : Set) : Set :=
 Arguments nil [T].
 Arguments cons [T].
 
+Notation "[]" := (nil).
+Notation "[ a ]" := (cons a nil).
+Notation "[ a ; b ; .. ; c ]" := (cons a (cons b .. (cons c nil) ..)).
+Notation "[ a ; .. ; b ]" := (cons a .. (cons b nil) ..).
+
 Fixpoint map (T T' : Set) (f : T -> T') (ls : list T) : list T' :=
   match ls with
-  | nil => nil
+  | [] => []
   | cons x ls' => cons (f x) (map f ls')
   end.
 
 Fixpoint filter (T : Set) (p : T -> bool) (ls : list T) : list T :=
   match ls with
-  | nil => nil
+  | [] => []
   | cons x ls' => if p x then cons x (filter p ls') else filter p ls'
+  end.
+
+Fixpoint mapPartial (T T' : Set) (f : T -> option T') (ls : list T) : list T' :=
+  match ls with
+  | nil => nil
+  | cons x ls' => match (f x) with
+                  | NONE => mapPartial f ls'
+                  | SOME y => cons y (mapPartial f ls')
+                  end
   end.
 
 Theorem map_fusion : forall (T T' T'' : Set) (f : T' -> T'')
                             (g : T -> T') (ls : list T),
-    map f (map g ls) = map (fun x => f (g x)) ls.
+    map f (map g ls) = map (f o g) ls.
   induction ls. reflexivity.
   simpl. rewrite <- IHls. reflexivity.
 Qed.
@@ -58,4 +87,9 @@ Lemma filter_fusion : forall (T : Set) (p q : T -> bool)
   reflexivity.
 Qed.
 
+Check compose'.
 
+Lemma mapPartial_fusion : forall (T T' T'' : Set) (f : T' -> option T'')
+                                 (g : T -> option T') (ls : list T),
+    ((mapPartial f) o (mapPartial g)) ls = mapPartial (f oo g) ls.
+  Proof.
